Fix last commit, which overwrite imp-terms instead of making new directory

coq/playground/term-simpl.v
@@ -6,33 +6,57 @@ Require Import Program.
 
 Set Implicit Arguments.
 
+Generalizable All Variables.
+
+Definition funty `(el : U -> Type) args res :=
+  fold_right  (fun a r => el a -> r) (el res) args.
+
+Definition funrel `(rels : forall (u : U), relation (el u))
+           args res : relation (funty el args res) :=
+ list_rect (fun args => relation (funty el args res))
+           (rels res) (fun a _ rs => respectful (rels a) rs) args.
+
+Definition funty' `(el : U -> Type) args res :=
+  fold_right  (fun a r => el a -> r) (option (el res)) args.
+
+Definition option_impl `(R : relation A) : relation (option A) :=
+  fun x y => match x, y with
+                | Some v, Some w => R v w
+                | None, _ => True
+                | _, _ => False
+              end.
+
+Definition funrel' `(rels : forall (u : U), relation (el u))
+           args res : relation (funty' el args res) :=
+ list_rect (fun args => relation (funty' el args res))
+           (option_impl (rels res)) (fun a _ rs => respectful (rels a) rs) args.
+
 Module Type Labels.
   Parameter sort : Set.
   Parameter domain : sort -> Set.
   Parameter domain_eq : forall s, relation (domain s).
   Parameter domain_eq_equiv : forall s, Equivalence (@domain_eq s).
+  Parameter label : Set.
+  Parameter label_args : label -> list sort.
+  Parameter label_res : label -> sort.
+  Parameter label_sem : forall l, funty' domain (label_args l) (label_res l).
+  Parameter label_proper : forall l, Proper (funrel' domain_eq (label_args l) (label_res l)) (label_sem l).
   Parameter var : sort -> Set.
 End Labels.
 
-Fixpoint funty {U : Set} (el : U -> Set) (args : list U) (res : U) : Set :=
-  match args with
-    | nil => el res
-    | (a :: args') => el a -> funty el args' res
-  end.
-
-Definition funty' {U : Set} (el el' : U -> Set) (args : list U) (res : U) : Set :=
-  @fold_right Set U (fun a r => el a -> r) (el' res) args.
-
 Module Terms (Import labels : Labels).
- 
-Definition label_ty args res := funty' domain (fun s => option (domain s)) args res.
-Inductive Term : forall s : sort, Set :=
+
+Definition label_ty args res := funty' domain args res.
+
+Unset Implicit Arguments.
+Inductive Term : forall s : sort, Type :=
  | TVar : forall {s}, var s -> Term s
- | TCon : forall {s args}, label_ty args s-> TArgs args -> Term s
-with TArgs : forall (args : list sort), Set :=
+ | TCon : forall l, TArgs (label_args l) -> Term (label_res l)
+with TArgs : forall (args : list sort), Type :=
  | TNil : TArgs nil
  | TCons : forall {a args}, Term a -> TArgs args -> TArgs (a :: args)
  .
+Set Implicit Arguments.
 
 Fixpoint gather {args : list sort} {res : sort} {struct args} :=
   match args as args return (TArgs args -> Term res) -> funty Term args res with
@@ -40,15 +64,14 @@ Fixpoint gather {args : list sort} {res : sort} {struct args} :=
     | (cons x xs) => fun k => fun x' => @gather xs _ (fun xs' => k (TCons x' xs'))
   end.
 
-Definition label (args : list sort) (res : sort) (f : label_ty args res) : funty Term args res :=
-  gather (TCon f).
+Definition lapply (l : label) := gather (TCon l).
 
 Notation Env := (forall s, var s -> option (domain s)).
 
 Fixpoint eval (env : Env) {s} (t : Term s) : option (domain s) :=
   match t with
     | TVar _ v => env _ v
-    | TCon _ _ f args => apply env (Some f) args
+    | TCon f args => apply env (Some (label_sem f)) args
   end
 with apply (env : Env) {args : list sort} {res : sort} (mf : option (label_ty args res))
            (ts : TArgs args){struct ts}  : option (domain res) :=
@@ -65,16 +88,23 @@ with apply (env : Env) {args : list sort} {res : sort} (mf : option (label_ty ar
       end f
   end.
 
-Definition option_rel (A : Set) (R : relation A) : relation (option A) :=
-  fun x y => match x, y with
-                | Some v, Some w => R v w
-                | None, None => True
-                | _, _ => False
-              end.
-
-Definition valid (s : sort) : relation (Term s) :=
+Definition valid_impl (s : sort) : relation (Term s) :=
   fun t1 t2 => forall env,
-                 option_rel (@domain_eq s) (eval env t1) (eval env t2).
+                 option_impl (@domain_eq s) (eval env t1) (eval env t2).
+
+Lemma valid_impl_refl (s : sort) : Reflexive (@valid_impl s).
+intro x; unfold valid_impl. intros. destruct (eval env x); simpl; reflexivity.
+Qed.
+Lemma valid_impl_trans (s : sort) : Transitive (@valid_impl s).
+intro x; unfold valid_impl. intros. specialize (H env).  specialize (H0 env).
+destruct (eval env x);destruct (eval env y);simpl in H;try tauto;destruct (eval env z);simpl in H0; try tauto.
+simpl. etransitivity;eassumption. 
+Qed.
+
+Add Parametric Relation (s : sort) : (Term s) (@valid_impl s)
+  reflexivity proved by (@valid_impl_refl s)
+  transitivity proved by (@valid_impl_trans s)
+  as valid_rel.
 
 Fixpoint valid_args (args : list sort) (ts1 : TArgs args) : TArgs args -> Prop :=
   match ts1 in TArgs args' return TArgs args' -> Prop with
@@ -89,23 +119,10 @@ Fixpoint valid_args (args : list sort) (ts1 : TArgs args) : TArgs args -> Prop :
                                        end with
           | TNil => I
           | TCons _ _ t2 ts2' => fun t1' ts1'' =>
-                                   valid t1' t2 /\ valid_args ts1'' ts2'
+                                   valid_impl t1' t2 /\ valid_args ts1'' ts2'
       end t1 ts1'
   end.
 
-Lemma valid_refl (s : sort) : Reflexive (@valid s).
-intro x; unfold valid. intros. destruct (eval env x); simpl; reflexivity.
-Qed.
-Lemma valid_trans (s : sort) : Transitive (@valid s).
-intro x; unfold valid. intros. specialize (H env).  specialize (H0 env).
-destruct (eval env x);destruct (eval env y);simpl in H;try tauto;destruct (eval env z);simpl in H0; try tauto.
-simpl. etransitivity;eassumption. 
-Qed.
-
-Add Parametric Relation (s : sort) : (Term s) (@valid s)
-  reflexivity proved by (@valid_refl s)
-  transitivity proved by (@valid_trans s)
-  as valid_rel.
 
 Ltac dep_dest_1 := let x := fresh "x" in intro x; dependent destruction x.
 Ltac straightforward_reflexivity := dep_dest_1; simpl; intuition reflexivity.
@@ -124,28 +141,22 @@ Add Parametric Relation (ss : list sort) : (TArgs ss) (@valid_args ss)
   as valid_args_rel.
 
 Add Parametric Morphism (s : sort) (ss : list sort) : (@TCons s ss)
-with signature (@valid s) ++> (@valid_args ss) ++> (@valid_args (s :: ss))
+with signature (@valid_impl s) ++> (@valid_args ss) ++> (@valid_args (s :: ss))
 as tcons_valid.
 simpl; auto.
 Qed.
 
-Fixpoint label_rel args res {struct args} : relation (label_ty args res) :=
-  match args as args return relation (label_ty args res) with
-    | nil => option_rel (@domain_eq res)
-    | a :: args' => (@domain_eq a ++> label_rel args' res)%signature
-   end.
-
 Lemma apply_rel
   (args : list sort)
   (res : sort)
-  (x : label_ty args res)
-  (y : label_ty args res)
-  (H : label_rel args res x y)
+  (x : funty' domain args res)
+  (y : funty' domain args res)
+  (H : funrel' domain_eq args res x y)
   (x0 : TArgs args)
   (y0 : TArgs args)
   (H0 : valid_args x0 y0) :
   forall env : Env,
-   option_rel (domain_eq (s:=res)) (apply env (Some x) x0)
+   option_impl (domain_eq (s:=res)) (apply env (Some x) x0)
      (apply env (Some y) y0).
 Proof.
 intro env.
@@ -157,17 +168,15 @@ simpl.
 destruct (eval env t);
 destruct (eval env t0);
 simpl in H0 |- *; try tauto.
-simpl in H.
-intuition.
+apply IHargs; auto.
 Qed.
 
-Add Parametric Morphism (args : list sort) (res : sort) : (@TCon res args)
-  with signature (label_rel args res) ++> (@valid_args args) ++> (@valid res)
+Add Parametric Morphism l : (TCon l)
+  with signature (@valid_args (label_args l)) ++> (@valid_impl (label_res l))
   as tcon_valid.
 Proof.
-intros; unfold valid; apply apply_rel; assumption.
+intros; unfold valid_impl; apply apply_rel; [apply label_proper |  assumption].
 Qed.
-
 End Terms.
 
 Module ExpLabel <: Labels.
@@ -180,10 +189,202 @@ Module ExpLabel <: Labels.
   Definition domain_eq s := @eq (domain s).
   Definition domain_eq_equiv s := @eq_equivalence (domain s).
   Definition var s := option (domain s).
+
+  Inductive labelI : Set :=
+    | lplus
+    | lcon (n : nat).
+  Definition label := labelI.
+  Definition label_args (l : labelI) :=
+    match l with
+      | lplus => [nsort ; nsort]
+      | lcon _ => nil
+    end.
+  Definition label_res (l : labelI) := nsort.
+  Definition label_sem (l : labelI) :=
+    match l as l return funty' domain (label_args l) (label_res l) with
+      | lplus => fun x y => Some (x + y)
+      | lcon v => Some v
+    end.
+  Definition label_proper (l : labelI) : Proper (funrel' domain_eq (label_args l) (label_res l)) (label_sem l).
+    destruct l; unfold Proper; simpl; unfold domain_eq, respectful; congruence.
+  Qed.
 End ExpLabel.
 
 Import ExpLabel.
 Module Import lterms := Terms ExpLabel.
+
+Notation tcon n := (TCon (lcon n) TNil : Term nsort).
+Notation tplus l r := (TCon lplus (TCons l (TCons r TNil)) : Term nsort).
+
+Lemma computing (x y : nat) : valid_impl (tplus (tcon x) (tcon y)) (tcon (x + y)).
+Proof.
+unfold valid_impl; reflexivity.
+Qed.
+Check computing.
+
+Lemma computing_r (x y : nat) : (Basics.flip (@valid_impl _)) (tplus (tcon x) (tcon y)) (tcon (x + y)).
+Proof.
+unfold flip, valid_impl; reflexivity.
+Qed.
+
+Lemma con_equiv (x y : nat) : x = y -> valid_impl (tcon x) (tcon y).
+congruence.
+Qed.
+
+Instance valid_default (s : sort) : DefaultRelation (@valid_impl s).
+Instance valids_default (ss : list sort) : DefaultRelation (@valid_args s).
+
+Fixpoint bu (simpl : forall s, Term s -> Term s) s (t : Term s) : Term s :=
+  match t in Term s' return Term s' with
+    | (TVar _ _ as t') => simpl _ t'
+    | TCon l args => simpl _ (TCon l (bus simpl args))
+  end
+with bus (simpl : forall s, Term s -> Term s) ss (ts : TArgs ss) : TArgs ss :=
+  match ts in TArgs ss' return TArgs ss' with
+    | TNil => TNil
+    | TCons _ _ t ts' => TCons (bu simpl t) (bus simpl ts')
+  end.
+
+Lemma bu_simpls : forall (simpl : forall s, Term s -> Term s)
+      (simpl_simpls : forall s (t : Term s), valid_impl t (simpl s t)),
+      forall s (t : Term s), valid_impl t (bu simpl t)
+with bus_simpls : forall (simpl : forall s, Term s -> Term s)
+      (simpl_simpls : forall s (t : Term s), valid_impl t (simpl s t)),
+      forall ss (ts : TArgs ss), valid_args ts (bus simpl ts).
+Proof.
+clear bu_simpls. destruct t;simpl;auto.
+rewrite <- simpl_simpls.
+auto using tcon_valid.
+
+clear bus_simpls. induction ts;simpl;auto.
+Qed.
+
+Definition simpl_plus s : Term s -> Term s :=
+ match s as s return Term s -> Term s with
+   | nsort => fun t => match t with
+                         | TCon lplus (TCons _ _ (TCon (lcon x) TNil)
+                                             (TCons _ _ (TCon (lcon y) TNil)
+                                                    TNil)) => TCon (lcon (x + y)) TNil
+                         | _ => t
+                       end
+ end.
+
+Lemma simpl_plus_simpls : forall s (t : Term s), valid_impl t (simpl_plus t).
+intros.
+destruct t.
+destruct s. reflexivity.
+destruct l; try reflexivity.
+dependent destruction t.
+dependent destruction t1.
+fold sort in t1.
+dependent destruction t1.
+dependent destruction t.
+reflexivity.
+destruct l.
+reflexivity.
+simpl in t.
+dependent destruction t.
+dependent destruction t2.
+reflexivity.
+destruct l.
+reflexivity.
+simpl in t.
+dependent destruction t.
+simpl.
+unfold valid_impl.
+simpl.
+reflexivity.
+Qed.
+
+Require Import Omega.
+
+Lemma test_computing (x y z : nat) :
+  valid_impl (tplus (tplus (tcon x) (tcon y)) (tcon z))
+             (tcon ((x + y) + z)).
+autounfold.
+rewrite computing.
+autounfold.
+rewrite computing.
+
+pose proof (computing (x + y) z).
+Set Printing All.
+autounfold.
+autounfold in H.
+rewrite H.
+Check trans_co_eq_inv_impl_morphism.
+Check
+(tcons_valid_Proper (computing x y) (TCons (tcon z) TNil) 
+          (TCons (tcon z) TNil)
+          (reflexive_proper_proxy
+             (valid_args_rel_Reflexive (ss:=[label_res (lcon z)]))
+             (TCons (tcon z) TNil)))
+.
+test_computing = 
+(fun
+   H : valid_impl (tplus (tcon (x + y)) (tcon z))
+         (tplus (tcon (x + y)) (tcon z)) =>
+ (fun lemma : valid_impl (tplus (tcon x) (tcon y)) (tcon (x + y)) =>
+  trans_co_eq_inv_impl_morphism (valid_rel_Transitive (s:=label_res lplus))
+    (tplus (tplus (tcon x) (tcon y)) (tcon z))
+    (tplus (tcon (x + y)) (tcon z))
+    (tcon_valid_Proper
+       (TCons (tplus (tcon x) (tcon y)) (TCons (tcon z) TNil))
+       (TCons (tcon (x + y)) (TCons (tcon z) TNil))
+       (tcons_valid_Proper lemma (TCons (tcon z) TNil) 
+          (TCons (tcon z) TNil)
+          (reflexive_proper_proxy
+             (valid_args_rel_Reflexive (ss:=[label_res (lcon z)]))
+             (TCons (tcon z) TNil)))) (tplus (tcon (x + y)) (tcon z))
+    (tplus (tcon (x + y)) (tcon z))
+    (eq_proper_proxy (Term (label_res lplus)) (tplus (tcon (x + y)) (tcon z))))
+   (computing x y) H) (reflexivity (tplus (tcon (x + y)) (tcon z)))
+     : forall x y z : nat,
+       valid_impl (tplus (tplus (tcon x) (tcon y)) (tcon z))
+         (tplus (tcon (x + y)) (tcon z))
+
+
+rewrite computing.
+reflexivity.
+Qed.
+Print test_computing.
+
+
+
+Lemma use_computing (x y z w : nat) :
+  valid_impl (tplus (tplus (tcon x) (tcon y)) (tplus (tcon z) (tcon w)))
+             (tplus (tcon x) (tplus (tplus (tcon y) (tcon z)) (tcon w))).
+Proof.
+assert 
+cut (valid_impl (tcon ((x + y) + (z + w)))
+                (tplus (tcon x) (tplus (tplus (tcon y) (tcon z)) (tcon w)))).
+rewrite computing.
+assert (Proper (valid_impl (s:=label_res lplus) ==> flip (@valid_impl (label_res lplus)) ==> flip impl)
+               (valid_impl (s:=label_res lplus))).
+unfold Proper.
+unfold flip.
+intro. intros.
+intro. intros.
+intro.
+transitivity y0. assumption.
+transitivity y1. assumption.
+assumption.
+
+Lemma 
+rewrite computing.
+rewrite computing.
+setoid_rewrite computing.
+
+rewrite (bu_simpls _ simpl_plus_simpls).
+simpl.
+congruence omega.
+setoid_rewrite computing.
+repeat match goal with [|- valid ?pre _] =>
+       match pre with context [tplus (tcon ?l) (tcon ?r)] => rewrite (computing l r) end end.
+repeat match goal with [|- valid _ ?post] =>
+       match post with context [tplus (tcon ?l) (tcon ?r)] => rewrite (computing_r l r) end end.
+apply con_equiv.
+omega.
+Qed.
 
 Definition oplus : label_ty (nsort :: nsort :: []) nsort  := fun x y => Some (x + y).
 
