coq/playground/himp/kstyle.v
@@ -1,0 +1,229 @@
+Add LoadPath "../../ml_proof".
+
+Require Import ZArith.
+Require Import List.
+Require Import FMapPositive.
+Require Import String.
+Open Scope string_scope.
+
+Require Import domains.
+
+Notation "'□' '+' e" := (Fplusl e) (at level 50) : k_scope.
+Notation "e '+' '□'" := (Fplusr e) (at level 50) : k_scope.
+Notation "'□' '/' e" := (Fdivl e) (at level 40): k_scope.
+Notation "e '/' '□'" := (Fdivr e) (at level 40): k_scope.
+Notation "'□' '<=' e" := (Flel e) (at level 70): k_scope.
+Notation "i '<=' '□'" := (Fler i) (at level 70): k_scope.
+Notation "'□' '&&' e" := (Fandl e) (at level 40): k_scope.
+Notation "v ':=□'" := (Fassign v) (at level 30): k_scope.
+Notation "'if□then' s1 'else' s2" := (Fif s1 s2) (at level 20): k_scope.
+
+Delimit Scope k_scope with K.
+Open Scope k_scope.
+
+Coercion KExp : Exp >-> kitem.
+Coercion KBExp : BExp >-> kitem.
+Coercion KStmt : Stmt >-> kitem.
+Coercion KFreezer : freezer >-> kitem.
+
+Set Implicit Arguments.
+
+Notation exp1_step step a b :=
+  (forall rest env henv, step (KCfg (kra a rest) env henv) 
+                              (KCfg (kra b rest) env henv)) (only parsing).
+Notation exp_step step a b :=
+  (forall env henv, step (KCfg a env henv) (KCfg b env henv)) (only parsing).
+
+Generalizable Variables rest env erest henv x y i j v r e b s.
+Inductive kstep : kcfg -> kcfg -> Prop :=
+  (* evaluation rules *)
+  | k_lookup : `(env = (x :-> i :* erest) ->
+                 kstep (KCfg (kra (EVar x) rest) env henv)
+                       (KCfg (kra (ECon i) rest) (x :-> i :* erest) henv))
+  | k_assign : `(env = (x :-> v :* erest) ->
+                 kstep (KCfg (kra (SAssign x (ECon i)) rest) env henv)
+                       (KCfg (kra Skip rest) (x :-> i :* erest) henv))
+  | k_plus : `(exp1_step kstep (EPlus (ECon i) (ECon j))
+                               (ECon (Zplus i j)))
+  | k_div : `(Zneq_bool 0%Z j = true ->
+               exp1_step kstep (EDiv (ECon i) (ECon j))
+                               (ECon (Zdiv i j)))
+  | k_le : `(exp1_step kstep (BLe (ECon i) (ECon j))
+                             (BCon (Zle_bool i j)))
+  | k_and_t : `(exp1_step kstep (BAnd (BCon true) b)
+                                b)
+  | k_and_f : `(exp1_step kstep (BAnd (BCon false) b)
+                                (BCon false))
+  | k_skip: `(exp_step kstep (kra Skip rest)
+                             rest)
+  | k_if_t : `(exp1_step kstep (SIf (BCon true) s1 s2)
+                               s1)
+  | k_if_f : `(exp1_step kstep (SIf (BCon false) s1 s2)
+                         s2)
+  | k_while : `(exp1_step kstep (SWhile b s)
+                                (SIf b (Seq s (SWhile b s)) Skip))
+  (* heating and cooling *)
+  (* plus *)
+  | k_heat_plus_l : `(isEVal e = false ->
+                exp_step kstep (kra (EPlus e e2) rest)
+                               (kra e (kra (□ + e2) rest)))
+  | k_heat_plus_r : `(isEVal e2 = false ->
+                exp_step kstep (kra (EPlus e e2) rest)
+                               (kra e2 (kra (e + □) rest)))
+  | k_cool_plus_l : `(exp_step kstep (kra (ECon i) (kra (□ + e) rest))
+                                     (kra (EPlus (ECon i) e) rest))
+  | k_cool_plus_r : `(exp_step kstep (kra (ECon i) (kra (e + □) rest))
+                                     (kra (EPlus e (ECon i)) rest))
+  (* div *)
+  | k_heat_div_l : `(isEVal e = false ->
+                exp_step kstep (kra (EDiv e e2) rest)
+                               (kra e (kra (□ / e2) rest)))
+  | k_heat_div_r : `(isEVal e2 = false ->
+                exp_step kstep (kra (EDiv e e2) rest)
+                               (kra e2 (kra (e / □) rest)))
+  | k_cool_div_l : `(exp_step kstep (kra (ECon i) (kra (□ / e) rest))
+                                    (kra (EDiv (ECon i) e) rest))
+  | k_cool_div_r : `(exp_step kstep (kra (ECon i) (kra (e / □) rest))
+                                    (kra (EDiv e (ECon i)) rest))
+  (* le is seqstrict *)
+  | k_heat_le_l : `(isEVal e = false ->
+                exp_step kstep (kra (BLe e e2) rest)
+                               (kra e (kra (□ <= e2) rest)))
+  | k_heat_le_r : `(isEVal e2 = false ->
+                exp_step kstep (kra (BLe (ECon i) e2) rest)
+                               (kra e2 (kra (i <= □) rest)))
+  | k_cool_le_l : `(exp_step kstep (kra (ECon i) (kra (□ <= e) rest))
+                                   (kra (BLe (ECon i) e) rest))
+  | k_cool_le_r : `(exp_step kstep (kra (ECon j) (kra (i <= □) rest))
+                                   (kra (BLe (ECon i) (ECon j)) rest))
+  (* and only left-strict *)
+  | k_heat_and : `(isBool b1 = false ->
+                 exp_step kstep (kra (BAnd b1 b2) rest)
+                                (kra b1 (kra (□ && b2) rest)))
+  | k_cool_and : `(exp_step kstep (kra (BCon b) (kra (□ && b2) rest))
+                                  (kra (BAnd (BCon b) b2) rest))
+  (* assign *)
+  | k_heat_assign : `(isEVal e = false ->
+                  exp_step kstep (kra (SAssign x e) rest)
+                                 (kra e (kra (x :=□) rest)))
+  | k_cool_assign : `(exp_step kstep (kra (ECon i) (kra (x :=□) rest))
+                                     (kra (SAssign x (ECon i)) rest))
+
+  (* if *)
+  | k_heat_if : `(isBool b = false ->
+               exp_step kstep (kra (SIf b s1 s2) rest)
+                              (kra b (kra (if□then s1 else s2) rest)))
+  | k_cool_if : `(
+               exp_step kstep (kra (BCon b) (kra (if□then s1 else s2) rest))
+                              (kra (SIf (BCon b) s1 s2) rest))
+  (* seq *)
+  | k_heat_seq : `(exp_step kstep (kra (Seq s1 s2) rest)
+                                  (kra s1 (kra s2 rest)))
+  .
+
+CoInductive steps : kcfg -> kcfg -> Prop :=
+  | done : forall c1 c2, c1 = c2 -> steps c1 c2
+  | more : forall c1 c2 c3, kstep c1 c2 -> steps c2 c3 -> steps c1 c3
+  .
+
+Ltac find x map k :=
+  match map with
+    | (x :-> _ :* _) => let pf := constr:(eq_refl map) in k pf
+    | (?mapl :* (x :-> ?v)) => let pf := constr:(mapComm mapl (x :-> v)) in k pf
+    | ?mapl :* ?mapr =>
+           find x mapl ltac:(fun pfl => let pf := constr:(eq_trans (f_equal (fun m => m :* mapr) pfl)
+                                                                   (mapAssoc (x :-> _) _ mapr))
+                                        in k pf)
+        || find x mapr ltac:(fun pfr => let pf := constr:(eq_trans (f_equal (fun m => mapl :* m) pfr)
+                                                                   (mapComAssoc mapl (x :-> _) _))
+                                        in k pf)
+  end.
+Ltac find_submap map submap k :=
+  match map with
+    | (submap :* _) => let pf := constr:(eq_refl map) in k pf
+    | (?mapl :* submap) => let pf := constr:(mapComm mapl submap) in k pf
+    | ?mapl :* ?mapr =>
+           find_submap mapl submap
+                       ltac:(fun pfl => let pf := constr:(eq_trans (f_equal (fun m => m :* mapr) pfl)
+                                                                   (mapAssoc submap _ mapr))
+                                        in k pf)
+        || find_submap mapr submap
+                       ltac:(fun pfr => let pf := constr:(eq_trans (f_equal (fun m => mapl :* m) pfr)
+                                                                   (mapComAssoc mapl submap _))
+                                        in k pf)
+  end.
+
+Ltac find_map_entry :=
+  match goal with
+    | [|- ?x :-> ?v = ?x :-> _ :* _] => rewrite <- (mapUnit (x :-> v)); reflexivity
+    | [|- ?map = ?x :-> ?v :* ?map2 ] =>
+      find x map ltac:(fun pf => exact pf)
+  end.
+
+Lemma mapUnitL : forall {A} (m : Map A), mapEmpty :* m = m.
+intros. rewrite mapComm. apply mapUnit.
+Qed.
+
+Ltac equate_maps := rewrite ?mapAssoc, ?mapUnitL, ?mapUnit;
+ repeat (rewrite ?f_equal;
+         match goal with
+           | [|- (?x :-> _ :* _) = (?x :-> _ :* _)] => apply f_equal2;[apply f_equal;omega|]
+           | [|-?map = ?x :-> _ :* _] => find x map ltac:(fun pf => rewrite pf)
+           | [|-?map = ?submap :* _] => find_submap map submap ltac:(fun pf => rewrite pf)
+           | [|- ?map = ?map ] => reflexivity
+         end).
+
+Ltac finish :=
+  apply done; apply (f_equal2 (KCfg _)); equate_maps.
+
+Lemma eval_happy : forall env,
+  steps (KCfg (kra (SAssign "x" (EPlus (EVar "x") (EVar "y"))) nil)
+            (env :* "x" :-> 12%Z :* "y" :-> 13%Z) mapEmpty)
+        (KCfg nil (env :* "x" :-> 25%Z :* "y" :-> 13%Z) mapEmpty).
+intros;
+repeat (eapply more;[econstructor (reflexivity || find_map_entry)|]).
+simpl Zplus;finish.
+Qed.
+
+Lemma loop_test:
+  steps (KCfg (kra (SWhile (BLe (ECon 0) (EVar "x"))
+    (SAssign "x" (EPlus (EVar "x") (ECon (-1)%Z))))
+  nil) ("x" :-> 25%Z) mapEmpty)
+  (KCfg nil ("x" :-> (-1)%Z) mapEmpty).
+Proof.
+intros;
+repeat (eapply more;[econstructor (reflexivity || find_map_entry)|];instantiate;simpl Zplus);
+finish.
+Qed.
+
+Ltac step_rule := eapply more;[econstructor (reflexivity || find_map_entry)|].
+Ltac split_if :=
+  match goal with
+      | [|- steps (KCfg (kra (KStmt (SIf (BCon (?x <=? ?y)%Z) _ _)) _) _ _) _] =>
+        pose proof (Zle_cases x y); destruct (x <=? y)%Z
+  end.
+
+Ltac use_circ circ :=
+  eapply circ;
+  try (match goal with [|- @eq (Map string) _ _] => equate_maps;reflexivity end);
+  instantiate;  omega.
+
+Ltac run_circ circ := repeat (use_circ circ || (step_rule || split_if || finish)).
+
+CoFixpoint sum :
+  forall (x y z : Z) erest env heap,
+    (0 <= x)%Z ->
+    z = (x + y)%Z ->
+    env = ("i" :-> x :* "j" :-> y :* erest) ->
+  steps
+    (KCfg (kra (SWhile (BLe (ECon 1%Z) (EVar "i"))
+                       (Seq
+                          (SAssign "i" (EPlus (EVar "i") (ECon (-1)%Z)))
+                          (SAssign "j" (EPlus (EVar "j") (ECon 1%Z)))))
+               kdot)
+                env heap)
+    (KCfg kdot
+          ("i" :-> 0%Z :* "j" :-> z%Z :* erest) heap).
+intros. subst env.
+step_rule; run_circ sum.
+Qed.
